#set text(size: 1.5em)
#set page(height: auto)

== Grundlagen

=== Bruchrechnung

$a / b + c / d = frac(a d + b c, b d)$

$a / b - c / d = frac(a d - b c, b d)$

$a / b dot.op c / d = frac(a c, b d)$

$(a / b) / (c / d) = frac(a dot.op d, b dot.op c)$

=== Potenzgesetze

$a^m dot.op a^n = a^(m + n)$

$a^m / a^n = a^(m - n)$

$(a^m)^n = a^(m dot.op n)$

$a^0 = 1 quad (a eq.not 0)$

$a^(- n) = 1 / a^n$

=== Wurzelgesetze

$sqrt(a dot.op b) = sqrt(a) dot.op sqrt(b)$

$sqrt(a / b) = sqrt(a) / sqrt(b)$

$root(n, a^m) = a^(m / n)$

=== Logarithmusgesetze

$log_a (x dot.op y) = log_a (x) + log_a (y)$

$log_a (x / y) = log_a (x) - log_a (y)$

$log_a (x^n) = n dot.op log_a (x)$

$log_a (x) = frac(log_b (x), log_b (a))$ (Basiswechsel)

=== Binomische Formeln

- $(a + b)^2 = a^2 + 2 a b + b^2$

- $(a - b)^2 = a^2 - 2 a b + b^2$

- $(a + b) (a - b) = a^2 - b^2$
